proof/modular_multiplication/BarretReduction_Concrete_CT.ec
@@ -1,0 +1,17 @@
+require import List Int AllCore. 
+require import W64_SchnorrExtract_ct.
+from Jasmin require import JModel.
+
+
+equiv bn_breduce_ct_equiv :
+  M(Syscall).bn_breduce ~ M(Syscall).bn_breduce :
+  ={M.leakages} ==> ={M.leakages}.
+proof.  proc. progress. inline*. sim. qed.
+
+lemma bn_breduce_ct &m r1 r2 a1 a2 p1 p2 l:
+  Pr[ M(Syscall).bn_breduce(r1,p1,a1)@&m: M.leakages = l ]
+    = Pr[ M(Syscall).bn_breduce(r2,p2,a2)@&m: M.leakages = l ].
+byequiv. conseq bn_breduce_ct_equiv. auto. auto. auto. auto.
+qed.
+
+
